theories/c_toy_lang/melocoton/class_instances.v
@@ -15,10 +15,6 @@ Section pure_exec.
     try destruct bool_decide eqn:H; 
     [apply bool_decide_eq_true_1 in H| apply bool_decide_eq_false_1 in H]).
 
-  Global Instance pure_let x (v1 v2 : val) :
-    PureExec True 1 p (Let x (Val v1) (Val v2)) (subst' x v1 v2).
-  Proof. solve_pure_exec. Qed.
-
   Global Instance pure_unop op v v' :
     PureExec (un_op_eval op v = Some v') 1 p (UnOp op (Val v)) (Val v').
   Proof. solve_pure_exec. Qed.
@@ -63,6 +59,10 @@ Section pure_exec.
 
   Global Instance pure_while e1 e2 : 
     PureExec True 1 p (While e1 e2) (If e1 (Let BAnon e1 (While e1 e2)) (Val $ LitV $ LitInt 0)).
+  Proof. solve_pure_exec. Qed.
+
+  Global Instance pure_let x (v1:val) e2 : 
+    PureExec True 1 p (Let x v1 e2) (subst' x v1 e2).
   Proof. solve_pure_exec. Qed.
 
   Global Instance pure_funcall s va args res e : 
