theories/c_toy_lang/melocoton/proofmode.v
@@ -10,12 +10,16 @@ Lemma tac_wp_expr_eval `{!heapGS Σ} Δ s E Φ e e' :
   envs_entails Δ (WP e' @ s; E {{ Φ }}) → envs_entails Δ (WP e @ s; E {{ Φ }}).
 Proof. by intros ->. Qed.
 
+
 Ltac solve_lookup_fixed := let rec go := match goal with
   [ |- context[ @lookup _ _ (@gmap _ ?eqdec _ _) _ ?needle (insert ?key ?val ?rem)]] =>
     (unify key needle; rewrite (@lookup_insert _ _ _ _ _ _ _ _ _ _ _ _ rem key val)) ||
     (rewrite (@lookup_insert_ne _ _ _ _ _ _ _ _ _ _ _ _ rem key needle val); [congruence|go])
+| [ |- context[ @lookup _ _ (@gmap _ ?eqdec _ _) _ ?needle (singletonM ?key ?val)]] =>
+    (unify key needle; rewrite (@lookup_singleton _ _ _ _ _ _ _ _ _ _ _ _ key val)) ||
+    (rewrite (@lookup_singleton_ne _ _ _ _ _ _ _ _ _ _ _ _ key needle val); congruence)
 | [ |- context[ @lookup _ _ (@gmap _ ?eqdec _ _) _ ?needle ∅]] => 
-    rewrite (@lookup_empty _ _  _ _ _ _ _ _ _ _ _ _ needle) end in repeat (progress (try go; simpl)).
+    rewrite (@lookup_empty _ _  _ _ _ _ _ _ _ _ _ _ needle) end in repeat (progress (unfold subst; try go; simpl)).
 
 Tactic Notation "wp_expr_eval" tactic3(t) :=
   iStartProof;
